src/SDK/Keyring/RawAESKeyring.dfy
@@ -104,7 +104,7 @@ module RawAESKeyring{
       requires Valid() 
       ensures Valid()
       ensures |edks| == 0 ==> res.Success? && res.value.None?
-      ensures res.Success? && res.value.Some? ==> res.value.get.encryptedDataKeys == edks
+      ensures res.Success? && res.value.Some? ==> Mat.ValidOnDecryptResult(algorithmSuiteID, encryptionContext, edks, res.value.get)
     {
       var i := 0;
       while i < |edks|
